Support C++ exceptions.

theories/lang/cpp/logic/const.v
@@ -28,8 +28,8 @@ Section defs.
 
   (* TODO this needs to be extended because if it is casting [volatile],
      then it needs to descend under [const] *)
-  Definition wp_const_body (wp_const : forall (from to : cQp.t) (addr : ptr) (ty : type) (Q : epred), mpred)
-    (tu : translation_unit) (from to : cQp.t)  (addr : ptr) (ty : type) (Q : epred) : mpred :=
+  Definition wp_const_body (wp_const : forall (from to : cQp.t) (addr : ptr) (ty : type) (Q : mpred), mpred)
+    (tu : translation_unit) (from to : cQp.t)  (addr : ptr) (ty : type) (Q : mpred) : mpred :=
     let '(cv, rty) := decompose_type ty in
     if q_const cv then Q
     else
@@ -113,7 +113,7 @@ Section defs.
   Axiom wp_const_intro : forall tu f t a ty Q, wp_const_body (wp_const tu) tu f t a ty Q |-- wp_const tu f t a ty Q.
 
   (* Sanity check the [_frame] property *)
-  Lemma fold_left_frame : forall B (l : list B) (f f' : epred -> B -> epred)  (Q Q' : epred),
+  Lemma fold_left_frame : forall B (l : list B) (f f' : mpred -> B -> mpred)  (Q Q' : mpred),
     (Q -* Q') |-- □ (Forall Q1 Q1' a, (Q1 -* Q1') -* (f Q1 a -* f' Q1' a)) -*  fold_left f l Q -* fold_left f' l Q'.
   Proof.
     move=>B l.
@@ -123,7 +123,7 @@ Section defs.
   Qed.
 
   (* Sanity check *)
-  Lemma wp_const_body_frame_uniform : forall CAST tu q q' p ty (Q Q' : epred),
+  Lemma wp_const_body_frame_uniform : forall CAST tu q q' p ty (Q Q' : mpred),
     Q -* Q'
     |-- □ (Forall a b p ty Q Q', (Q -* Q') -* CAST a b p ty Q -* CAST a b p ty Q') -*
         wp_const_body CAST tu q q' p ty Q -* wp_const_body CAST tu q q' p ty Q'.
@@ -178,7 +178,7 @@ Section defs.
   Qed.
 
   (*
-  Lemma cv_cast_body_frame : forall CAST CAST' tu tu' q q' p ty (Q Q' : epred),
+  Lemma cv_cast_body_frame : forall CAST CAST' tu tu' q q' p ty (Q Q' : mpred),
     sub_module tu tu' ->
         Q -* Q'
     |-- □ (Forall a b p ty Q Q', (Q -* Q') -* CAST a b p ty Q -* CAST' a b p ty Q') -*
