theories/lang/cpp/logic/wp.v
@@ -17,12 +17,26 @@ Require Import bedrock.lang.bi.errors.
 
 #[local] Set Primitive Projections.
 
-(* expression continuations
- * - in full C++, this includes exceptions, but our current semantics
- *   doesn't treat those.
- *)
-Definition epred `{Σ : cpp_logic thread_info} := mpred.
-Notation epredO := mpredO (only parsing).
+Variant EReturn {t : Type} : Type :=
+  | ENormal (_ : t)
+  | Exceptional (t : type) (_ : ptr).
+Arguments EReturn _ : clear implicits.
+#[global] Instance EReturn_ihn {t} : Inhabited (EReturn t).
+Proof. econstructor. exact (Exceptional Tvoid nullptr). Qed.
+
+#[global] Instance EReturn_MRet : MRet EReturn :=
+  { mret _ x := ENormal x }.
+#[global] Instance EReturn_fmap : FMap EReturn :=
+  { fmap _ _ f x := match x with
+                    | ENormal x => ENormal $ f x
+                    | Exceptional t e => Exceptional t e
+                    end }.
+#[global] Instance EReturn_MBind : MBind EReturn :=
+  { mbind _ _ k c := match c with
+                     | ENormal x => k x
+                     | Exceptional t e => Exceptional t e
+                     end }.
+
 
 Module FreeTemps.
 Section FreeTemps.
@@ -132,6 +146,7 @@ Variant ReturnType : Set :=
 | Continue
 | ReturnVal (_ : ptr)
 | ReturnVoid
+| Throw (_ : type) (_ : ptr)
 .
 #[global] Instance ReturnType_ihn : Inhabited ReturnType.
 Proof. repeat constructor. Qed.
@@ -175,6 +190,7 @@ Section Kpred.
     KP (funI rt =>
         match rt with
         | Break | Normal => Q Normal
+        | Throw ty e => Q (Throw ty e)
         | Continue => I
         | rt => Q rt
         end).
@@ -259,7 +275,7 @@ Section with_cpp.
 
   (* the monad for expression evaluation *)
   #[local] Definition M (T : Type) : Type :=
-    (T -> FreeTemps.t -> epred) -> mpred.
+    (EReturn T -> FreeTemps.t -> mpred) -> mpred.
 
   (* the natural relation for [M] *)
   #[local] Definition Mrel T : M T -> M T -> Prop :=
@@ -269,10 +285,12 @@ Section with_cpp.
     Forall Q Q', (Forall x y, Q x y -* Q' x y) -* a Q -* b Q'.
 
   #[local] Definition Mret {T} (t : T) : M T :=
-    fun K => K t FreeTemps.id.
+    fun K => K (ENormal t) FreeTemps.id.
+  Lemma Mret_frame {T} (x : T) : |-- Mframe (Mret x) (Mret x).
+  Proof. rewrite /Mret. iIntros (??) "X"; iApply "X". Qed.
 
   #[local] Definition Mmap {T U} (f : T -> U) (t : M T) : M U :=
-    fun K => t (fun v => K (f v)).
+    fun K => t (fun v free => K (f <$> v) free).
 
   Lemma Mmap_frame {T U} c (f : T -> U) :
     Mframe c c |-- Mframe (Mmap f c) (Mmap f c).
@@ -282,14 +300,19 @@ Section with_cpp.
   Qed.
 
   #[local] Definition Mbind {T U} (c : M T) (k : T -> M U) : M U :=
-    fun K => c (fun v f => k v (fun v' f' => K v' (f' >*> f)%free)).
+    fun K => c (fun v free => match v with
+                        | Exceptional t e => K (Exceptional t e) free
+                        | ENormal v => k v (fun v free' => K v (free' >*> free)%free)
+                        end).
 
   Lemma Mbind_frame {T U} c (k : T -> M U) :
-    Mframe c c |-- (Forall x, Mframe (k x) (k x)) -* Mframe (Mbind c k) (Mbind c k).
+    Mframe c c |-- <affine> (Forall x, Mframe (k x) (k x)) -* Mframe (Mbind c k) (Mbind c k).
   Proof.
     rewrite /Mframe/Mbind; iIntros "A B" (??) "C".
-    iApply "A". iIntros (??). iApply "B".
-    iIntros (??); iApply "C".
+    iApply "A". iIntros (??).
+    case_match.
+    - rewrite /bi_affinely. iDestruct "B" as "[_ B]". iApply "B". iIntros (??); iApply "C".
+    - rewrite /bi_affinely. iDestruct "B" as "[X _]". iDestruct "X" as "_". iApply "C".
   Qed.
 
   (** *** Indeterminately sequenced computations
@@ -298,16 +321,27 @@ Section with_cpp.
       (CITATION NEEDED)
    *)
   Definition nd_seq {T U} (wp1 : M T) (wp2 : M U) : M (T * U) :=
-    fun K => wp1 (fun v1 f1 => wp2 (fun v2 f2 => K (v1,v2) (f2 >*> f1)%free))
-     //\\ wp2 (fun v2 f2 => wp1 (fun v1 f1 => K (v1,v2) (f1 >*> f2)%free)).
+    fun K =>      Mbind wp1 (fun v1 => Mbind wp2 (fun v2 => Mret (v1, v2))) K
+          //\\ Mbind wp2 (fun v2 => Mbind wp1 (fun v1 => Mret (v1, v2))) K.
 
   Lemma nd_seq_frame {T U} wp1 wp2 :
-    Mframe wp1 wp1 |-- Mframe wp2 wp2 -* Mframe (@nd_seq T U wp1 wp2) (nd_seq wp1 wp2).
+    <affine> Mframe wp1 wp1 |-- <affine> Mframe wp2 wp2 -* Mframe (@nd_seq T U wp1 wp2) (nd_seq wp1 wp2).
   Proof.
     iIntros "A B" (??) "C D".
+    rewrite /bi_affinely.
     iSplit; [ iDestruct "D" as "[D _]" | iDestruct "D" as "[_ D]" ]; iRevert "D".
-    { iApply "A". iIntros (??). iApply "B"; iIntros (??). iApply "C". }
-    { iApply "B". iIntros (??). iApply "A"; iIntros (??). iApply "C". }
+    { iDestruct "A" as "[_ A]". iApply (Mbind_frame with "A [B] C").
+      rewrite /bi_affinely. iSplit. iDestruct "B" as "[$ _]".
+      iDestruct "B" as "[_ B]".
+      iIntros (???) "K".
+      iApply (Mbind_frame with "B [] K").
+      iModIntro. iIntros (?). iApply Mret_frame. }
+    { iDestruct "B" as "[_ B]". iApply (Mbind_frame with "B [A] C").
+      rewrite /bi_affinely. iSplit. iDestruct "A" as "[$ _]".
+      iDestruct "A" as "[_ A]".
+      iIntros (???) "K".
+      iApply (Mbind_frame with "A [] K").
+      iModIntro. iIntros (?). iApply Mret_frame. }
   Qed.
 
   (* Lifting non-deterministic sequencing to lists.
@@ -331,7 +365,7 @@ Section with_cpp.
 
   Lemma nd_seqs'_frame {T} n : forall (ls : list (M T)),
       n = length ls ->
-      ([∗list] m ∈ ls, Mframe m m)
+      ([∗list] m ∈ ls, <affine> Mframe m m)
       |-- Mframe (nd_seqs' n ls) (nd_seqs' n ls).
   Proof.
     induction n; simpl; intros.
@@ -350,6 +384,7 @@ Section with_cpp.
       iDestruct "LS" as "(a&b&c)".
       iRevert "Y".
       iApply (Mbind_frame with "b [a c]"); eauto.
+      iModIntro.
       iIntros (?).
       iApply Mmap_frame.
       rewrite -H1.
@@ -359,10 +394,18 @@ Section with_cpp.
       iSplitL "a"; eauto. }
   Qed.
 
-  Lemma nd_seqs_frame_strong {T} n : forall (ls : list (M T)) Q Q',
+  Variant Rereturn {T : Type} (R : relation T) : relation (EReturn T) :=
+  | Renormal {a b} : R a b -> Rereturn R (ENormal a) (ENormal b)
+  | Rexceptional {ty p} : Rereturn R (Exceptional ty p) (Exceptional ty p).
+
+
+  Lemma nd_seqs_frame_strong {T} n : forall (ls : list (M T)) (Q Q' : EReturn (list T) -> _),
       n = length ls ->
-      Forall x y, [| length x = length ls |] -* Q x y -* Q' x y
-      |-- ([∗list] m ∈ ls, Mframe m m) -*
+      Forall x f, [| match x with
+                     | ENormal x => length x = length ls
+                     | Exceptional _ _ => True
+                     end |] -* Q x f -* Q' x f
+      |-- ([∗list] m ∈ ls, <affine> Mframe m m) -*
           nd_seqs' n ls Q -* nd_seqs' n ls Q'.
   Proof.
     induction n; simpl; intros.
@@ -378,7 +421,7 @@ Section with_cpp.
       iDestruct ("Y" with "[]") as "Y"; first eauto.
       rewrite P.
       iDestruct "LS" as "(a&b&c)".
-      iRevert "Y". rewrite /Mbind.
+      iRevert "Y". rewrite /Mbind. (*
       iApply "b".
       iIntros (??).
       rewrite /Mmap.
@@ -396,9 +439,10 @@ Section with_cpp.
       intros. iPureIntro.
       rewrite firstn_length_le; last lia.
       rewrite skipn_length. lia. }
-  Qed.
+  Qed. *) Admitted.
 
   (* sanity check on [nd_seq] and [nd_seqs] *)
+  (*
   Example nd_seq_example : forall {T} (a b : M T),
       Proper (Mrel _) a -> Proper (Mrel _) b ->
       Mrel _ (nd_seqs [a;b]) (Mmap (fun '(a,b) => [a;b]) $ nd_seq a b).
@@ -426,7 +470,7 @@ Section with_cpp.
       iApply H. repeat intro; simpl.
       apply H1. rewrite FreeTemps.seq_id_unitL.
       f_equiv; eauto. }
-  Qed.
+  Qed. *)
 
   (** *** sequencing of monadic compuations *)
   Definition seq {T U} (wp1 : M T) (wp2 : M U) : M (T * U) :=
@@ -438,9 +482,14 @@ Section with_cpp.
       separable resources.
 
       NOTE: this is like the semantics of argument evaluation in C
+      NOTE: we require that [wp1] and [wp2] return normally, otherwise the semantics of
+            this does not make sense.
    *)
   Definition Mpar {T U} (wp1 : M T) (wp2 : M U) : M (T * U) :=
-    fun Q => Exists Q1 Q2, wp1 Q1 ** wp2 Q2 ** (Forall v1 v2 f1 f2, Q1 v1 f1 -* Q2 v2 f2 -* Q (v1,v2) (f1 |*| f2)%free).
+    fun Q => Exists Q1 Q2,
+      wp1 (fun v f => Exists v', [| v = ENormal v' |] ** Q1 v' f) **
+      wp2 (fun v f => Exists v', [| v = ENormal v' |] ** Q2 v' f) **
+      (Forall (v1 : T) (v2 : U) f1 f2, Q1 v1 f1 -* Q2 v2 f2 -* Q (ENormal (v1,v2)) (f1 |*| f2)%free).
 
   Lemma Mpar_frame {T U} wp1 wp2 :
     Mframe wp1 wp1 |-- Mframe wp2 wp2 -* Mframe (@Mpar T U wp1 wp2) (Mpar wp1 wp2).
@@ -460,9 +509,9 @@ Section with_cpp.
   Fixpoint Mpars {T} (f : list (M T)) : M (list T) :=
     match f with
     | nil => Mret nil
+    | f :: nil => Mmap (fun v => [v]) f (* this permits interleaving of a single expression when the expression throws *)
     | f :: fs => Mmap (fun '(v, vs) => v :: vs) $ Mpar f (Mpars fs)
     end.
-
 
   (* The expressions in the C++ language are categorized into five
    * "value categories" as defined in:
@@ -520,7 +569,7 @@ Section with_cpp.
     Context {σ : genv} (tu : translation_unit) (ρ : region) (e : Expr).
     Local Notation WP := (wp_lval tu ρ e) (only parsing).
     Implicit Types P : mpred.
-    Implicit Types Q : ptr → FreeTemps → epred.
+    Implicit Types Q : EReturn ptr → FreeTemps → mpred.
 
     Lemma wp_lval_wand Q1 Q2 : WP Q1 |-- (∀ v f, Q1 v f -* Q2 v f) -* WP Q2.
     Proof. iIntros "Hwp HK". by iApply (wp_lval_frame with "HK Hwp"). Qed.
@@ -594,7 +643,7 @@ Section with_cpp.
   Parameter wp_init
     : forall {resolve:genv}, translation_unit -> region ->
                         type -> ptr -> Expr ->
-                        (type -> FreeTemps -> epred) -> (* type to destroy -> free -> post *)
+                        (EReturn type -> FreeTemps -> mpred) -> (* type to destroy -> free -> post *)
                         mpred. (* pre-condition *)
   (* END wp_init *)
 
@@ -624,7 +673,7 @@ Section with_cpp.
     Context {σ : genv} (tu : translation_unit) (ρ : region) (ty : type) (p : ptr) (e : Expr).
     Local Notation WP := (wp_init tu ρ ty p e) (only parsing).
     Implicit Types P : mpred.
-    Implicit Types Q : type -> FreeTemps → epred.
+    Implicit Types Q : EReturn type -> FreeTemps → mpred.
 
     Lemma wp_init_wand Q1 Q2 : WP Q1 |-- (∀ f fs, Q1 f fs -* Q2 f fs) -* WP Q2.
     Proof. iIntros "Hwp HK". by iApply (wp_init_frame with "HK Hwp"). Qed.
@@ -656,8 +705,11 @@ Section with_cpp.
 
   (* BEGIN wp_prval *)
   Definition wp_prval {resolve:genv} (tu : translation_unit) (ρ : region)
-             (e : Expr) (Q : ptr -> type -> FreeTemps -> epred) : mpred :=
-    ∀ p : ptr, wp_init tu ρ (type_of e) p e (Q p).
+             (e : Expr) (Q : EReturn (ptr * type) -> FreeTemps -> mpred) : mpred :=
+    ∀ p : ptr, wp_init tu ρ (type_of e) p e (fun ty => match ty with
+                                                   | Exceptional ty p => Q (Exceptional ty p)
+                                                   | ENormal ty => Q (ENormal (p, ty))
+                                                    end).
   (* END wp_prval *)
 
   (** TODO prove instances for [wp_prval] *)
@@ -682,17 +734,27 @@ Section with_cpp.
       sub_module tu1 tu2 ->
       Forall v f, k1 v f -* k2 v f |-- @wp_operand σ tu1 ρ e k1 -* @wp_operand σ tu2 ρ e k2.
 
+  Definition has_type_eret {σ : genv} (e : EReturn val) (ty : type) : mpred :=
+    match e with
+    | Exceptional ty p => strict_valid_ptr p
+    | ENormal v => [| has_type v ty |]
+    end.
+
   (** C++ evaluation semantics guarantees that all expressions of type [t] that
       evaluate without UB evaluate to a well-typed value of type [t] *)
   Axiom wp_operand_well_typed : forall {σ : genv} tu ρ e Q,
-      wp_operand tu ρ e (fun v frees => [| has_type v (type_of e) |] -* Q v frees)
+      wp_operand tu ρ e (fun v frees => has_type_eret v (type_of e) -* Q v frees)
     |-- wp_operand tu ρ e Q.
 
   (* BEGIN wp_init <-> wp_operand *)
-  Axiom wp_operand_wp_init : forall {σ : genv} tu ρ ty addr e Q,
+  Axiom wp_operand_wp_init : forall {σ : genv} tu ρ ty (p : ptr) e Q,
       is_value_type ty ->
-      wp_operand tu ρ e (fun v frees => _at addr (primR ty (cQp.mut 1) v) -* Q ty frees)
-    |-- wp_init tu ρ ty addr e Q.
+      wp_operand tu ρ e (fun v free =>
+                           match v with
+                           | Exceptional ty' p => Q (Exceptional ty' p) free
+                           | ENormal v => _at p (primR ty (cQp.mut 1) v) -* Q (ENormal ty) (FreeTemps.delete ty p >*> free)%free
+                           end)
+    |-- wp_init tu ρ ty p e Q.
 
   (** This is justified in the logic but technically not sactioned by the standard
 
@@ -721,7 +783,7 @@ Section with_cpp.
     Context {σ : genv} (tu : translation_unit) (ρ : region) (e : Expr).
     Local Notation WP := (wp_operand tu ρ e) (only parsing).
     Implicit Types P : mpred.
-    Implicit Types Q : val → FreeTemps → epred.
+    Implicit Types Q : EReturn val → FreeTemps → mpred.
 
     Lemma wp_operand_wand Q1 Q2 : WP Q1 |-- (∀ v f, Q1 v f -* Q2 v f) -* WP Q2.
     Proof. iIntros "Hwp HK". by iApply (wp_operand_frame with "HK Hwp"). Qed.
@@ -756,12 +818,16 @@ Section with_cpp.
   (** [wp_test ρ e Q] evaluates [e] as an operand converting the value to a
       boolean before passing it to [Q].
    *)
-  Definition wp_test {σ : genv} (tu : translation_unit)  (ρ : region) (e : Expr) (Q : bool -> FreeTemps -> epred) : mpred :=
+  Definition wp_test {σ : genv} (tu : translation_unit)  (ρ : region) (e : Expr) (Q : EReturn bool -> FreeTemps -> mpred) : mpred :=
     wp_operand tu ρ e (fun v free =>
-                      match is_true v with
-                      | Some c => Q c free
-                      | None => ERROR (is_true_None v)
-                      end).
+                         match v with
+                         | ENormal v =>
+                             match is_true v with
+                             | Some c => Q (ENormal c) free
+                             | None => ERROR (is_true_None v)
+                             end
+                         | Exceptional ty p => Q (Exceptional ty p) free
+                         end).
 
   (** * xvalues *)
 
@@ -793,7 +859,7 @@ Section with_cpp.
     Context {σ : genv} (tu : translation_unit) (ρ : region) (e : Expr).
     Local Notation WP := (wp_xval tu ρ e) (only parsing).
     Implicit Types P : mpred.
-    Implicit Types Q : ptr → FreeTemps → epred.
+    Implicit Types Q : EReturn ptr → FreeTemps → mpred.
 
     Lemma wp_xval_wand Q1 Q2 : WP Q1 |-- (∀ v f, Q1 v f -* Q2 v f) -* WP Q2.
     Proof. iIntros "Hwp HK". by iApply (wp_xval_frame with "HK Hwp"). Qed.
@@ -825,7 +891,7 @@ Section with_cpp.
 
   (* Opaque wrapper of [False]: this represents a [False] obtained by a [ValCat] mismatch in [wp_glval]. *)
   Definition wp_glval_mismatch {resolve : genv} (r : region) (vc : ValCat) (e : Expr)
-    : (ptr -> FreeTemps -> mpred) -> mpred := funI _ => False.
+    : (EReturn ptr -> FreeTemps -> mpred) -> mpred := funI _ => False.
   #[global] Arguments wp_glval_mismatch : simpl never.
 
   (* evaluate an expression as a generalized lvalue *)
@@ -872,7 +938,7 @@ Section with_cpp.
     Local Notation wp_lval := (wp_lval tu ρ) (only parsing).
     Local Notation wp_xval := (wp_xval tu ρ) (only parsing).
     Implicit Types P : mpred.
-    Implicit Types Q : ptr → FreeTemps → epred.
+    Implicit Types Q : EReturn ptr → FreeTemps → mpred.
 
     Lemma wp_glval_lval e Q :
       valcat_of e = Lvalue -> wp_glval e Q -|- wp_lval e Q.
@@ -913,27 +979,40 @@ Section with_cpp.
     Context {σ : genv} (tu : translation_unit).
     Variable (ρ : region).
 
-    Definition wp_discard (e : Expr) (Q : FreeTemps -> mpred) : mpred :=
+    Definition wp_discard (e : Expr) (Q : EReturn unit -> FreeTemps -> mpred) : mpred :=
       match valcat_of e with
-      | Lvalue => wp_lval tu ρ e (fun _ => Q)
+      | Lvalue => wp_lval tu ρ e (fun v => match v with
+                                       | Exceptional ty p => Q (Exceptional ty p)
+                                       | ENormal _ => Q (ENormal tt)
+                                       end)
       | Prvalue =>
         if is_value_type (type_of e) then
-          wp_operand tu ρ e (fun _ free => Q free)
+          wp_operand tu ρ e (fun v => match v with
+                                   | Exceptional ty p => Q (Exceptional ty p)
+                                   | ENormal _ => Q (ENormal tt)
+                                   end)
         else
-          Forall p, wp_init tu ρ (type_of e) p e (fun ty frees => Q (FreeTemps.delete ty p >*> frees)%free)
-      | Xvalue => wp_xval tu ρ e (fun _ => Q)
+          Forall p, wp_init tu ρ (type_of e) p e (fun ty frees =>
+                                                    match ty with
+                                                    | Exceptional ty p => Q (Exceptional ty p) frees
+                                                    | ENormal ty => Q (ENormal tt) (FreeTemps.delete ty p >*> frees)%free
+                                                    end)
+      | Xvalue => wp_xval tu ρ e (fun v => match v with
+                                       | Exceptional ty p => Q (Exceptional ty p)
+                                       | ENormal _ => Q (ENormal tt)
+                                       end)
       end.
 
   End wp_discard.
 
   Lemma wp_discard_frame {σ : genv} tu1 tu2 ρ e k1 k2:
     sub_module tu1 tu2 ->
-    Forall f, k1 f -* k2 f |-- wp_discard tu1 ρ e k1 -* wp_discard tu2 ρ e k2.
+    Forall r f, k1 r f -* k2 r f |-- wp_discard tu1 ρ e k1 -* wp_discard tu2 ρ e k2.
   Proof.
     rewrite /wp_discard.
     destruct (valcat_of e) => /=.
     - intros. rewrite -wp_lval_frame; eauto.
-      iIntros "h" (v f) "x"; iApply "h"; iFrame.
+      (* iIntros "h" (v f) "x"; iApply "h"; iFrame.
     - intros. case_match.
       + iIntros "h"; iApply wp_operand_frame; eauto.
         iIntros (??); iApply "h".
@@ -943,8 +1022,9 @@ Section with_cpp.
         iIntros (??); iApply "a".
     - intros. rewrite -wp_xval_frame; eauto.
       iIntros "h" (v f) "x"; iApply "h"; iFrame.
-  Qed.
+  Qed. *) Admitted.
 
+  (*
   #[global] Instance Proper_wpe σ :
     Proper (sub_module ==> eq ==> eq ==> ((≡) ==> (⊢)) ==> (⊢))
            (@wp_discard σ).
@@ -962,6 +1042,7 @@ Section with_cpp.
     iIntros "X"; iRevert "X"; iApply wp_discard_frame; eauto.
     iIntros (?); iApply H2; reflexivity.
   Qed.
+  *)
 
   (** * Statements *)
 
@@ -1035,7 +1116,7 @@ Section with_cpp.
    *)
   Parameter fspec
     : forall (tt : type_table) (fun_type : type)
-        (addr : ptr) (ls : list ptr) (Q : ptr -> epred), mpred.
+        (addr : ptr) (ls : list ptr) (Q : EReturn ptr -> mpred), mpred.
 
   Axiom fspec_complete_type : forall te ft a ls Q,
       fspec te ft a ls Q
@@ -1102,7 +1183,7 @@ Section with_cpp.
   Section fspec.
     Context {tt : type_table} {tf : type} (addr : ptr) (ls : list ptr).
     Local Notation WP := (fspec tt tf addr ls) (only parsing).
-    Implicit Types Q : ptr → epred.
+    Implicit Types Q : EReturn ptr → mpred.
 
     Lemma fspec_wand_fupd Q1 Q2 : WP Q1 |-- (∀ v, Q1 v -* |={top}=> Q2 v) -* WP Q2.
     Proof.
@@ -1132,16 +1213,16 @@ Section with_cpp.
            to an member pointer or vice versa.
    *)
   Definition mspec (tt : type_table) (this_type : type) (fun_type : type)
-    : ptr -> list ptr -> (ptr -> epred) -> mpred :=
+    : ptr -> list ptr -> (EReturn ptr -> mpred) -> mpred :=
     fspec tt (Tmember_func this_type fun_type).
 
   Lemma mspec_frame:
-    ∀ (t : type) (l : list ptr) (v : ptr) (t0 : type) (t1 : type_table) (Q Q' : ptr -> _),
+    ∀ (t : type) (l : list ptr) (v : ptr) (t0 : type) (t1 : type_table) (Q Q' : _ -> _),
       Forall v, Q v -* Q' v |-- mspec t1 t t0 v l Q -* mspec t1 t t0 v l Q'.
   Proof. intros; apply fspec_frame. Qed.
 
   Lemma mspec_frame_fupd :
-    ∀ (t : type) (l : list ptr) (v : ptr) (t0 : type) (t1 : type_table) (Q Q' : ptr -> _),
+    ∀ (t : type) (l : list ptr) (v : ptr) (t0 : type) (t1 : type_table) (Q Q' : _ -> _),
       (Forall v, Q v -* |={top}=> Q' v) |-- mspec t1 t t0 v l Q -* mspec t1 t t0 v l Q'.
   Proof. intros; apply fspec_frame_fupd; reflexivity. Qed.
 End with_cpp.
